# Differential Equations
> A differential equation is an equation which contains one or more terms and the derivatives of one variable (i.e., dependent variable) with respect to the other variable

Differential equations are classified by **type, order and linearity**.

An **ordinary differential equation** (ODE) is an equation containing an unknown function of **one** real or complex variable x, its derivatives, and some given functions of x. The unknown function is generally represented by a variable (often denoted y), which, therefore, depends on x. Thus x is often called the *independent variable* of the equation. E.g.:  
$$\begin{align}
&\frac{dy}{dt}-5y=1\space\space\space &(1)
\\\\
&\frac{du}{dx}-\frac{dv}{dx}=x\space\space\space &(2)
\\\\
&\frac{d^2y}{dx^2}-2\frac{dy}{dx}+6=0\space\space\space &(3)
\end{align}$$

If the equation involves partial derivatives, with relation to two or more independent variables, it is called **partial differential equation**.
E.g.:

$$\begin{align}
&\frac{\partial u}{\partial y} = \frac{\partial v}{\partial x} &(1)
\\\\
&x\frac{\partial u}{\partial x} + \frac{\partial u}{\partial y}=y &(2)
\end{align}$$


The **order of the equation** is simply the order of the biggest derivative in it. E.g.: $\frac{d^2y}{dx^2}+5=e^x$ is an 2nd order differential equation.

A differential equation is called linear when it can be rewritten as:
$$
a_n(x)\frac{d^ny}{dx^n}+ a_{n-1}(x)\frac{d^{n-1}y}{dx^{n-1}}+\dots + a_1(x)\frac{dy}{dx} + a_0(x)y = g(x)
$$

And it is characterized by the following properties:
- the dependent variable y and all it's derivatives are of first order
- each coefficient depends only on the independent variable x
E.g.:
$$\begin{align*}
&xdy + ydx = 0 &(1) 
\\ 
&y'' - 2y' + y = 0 &(2)
\\
&x^3\frac{d^3y}{dx^3}-x^2\frac{d^2y}{dx^2}+3x\frac{du}{dx}+5y=e^x &(3)
\end{align*}$$

Any equation $y=f(x)$, that, put into the differential equation, reduces it to an identity, is called a solution to the equation. E.g.:


$$\begin{align}
&y\frac{x^4}{16}\rightarrow y\prime=xy^{1/2} &(1)
\\\\
&y=xe^x \rightarrow y\prime\prime-2y\prime+y=0 &(2)
\end{align}$$
Linear differential equations can be taken from the _time domain_ to the _complex domain_ to be solved as algebraic equations using the [[Laplace Transform]].


mermaid
flowchart TD

A[DE in the time domain] --> B[DE Transformed by Laplace
now in S domain] --> C[Inverse Laplace Transform

DE back to time domain] --> Solution

##### Problem 1. 

**Find the solution for: $y'=xy^{1/2}$**


$$\begin{align}
&y^{1/2} = \sqrt{y} &(1)
\\
&\frac{dy}{dx} = x\sqrt{y} &(2)
\end{align}$$
To isolate x and y we can treat $dy/dx$ as a common fraction.

$$\begin{align}
&dy = x\sqrt{y}\space dx &(3)
\\
&\frac{dy}{\sqrt{y}}=xdx &(4)
\\
\\
&\int y^{-1/2}dy=\int xdx &(5)
\\
&\int y^{-1/2}dy =2\sqrt{y} &(6)
\\
&2\sqrt{y}=\frac{x^2}{2}+C &(7)
\\
&\sqrt{y}=(\frac{x^2}{4}+\frac{C}{2}), \space \frac{C}{2}=K &(7)
\\
&y = (\frac{x^2}{4}+k)^2 &(9)
\\
&\text{or as a general solution: }y=\frac{x^4}{16} &(9)
\end{align}$$




##### Problem 2
Here’s the same answer with the questions in LaTeX code blocks:

---

### Step 1: Write the Differential Equation
The given differential equation is:


$$
\frac{d^2 y(t)}{dt^2} + 5 \frac{dy(t)}{dt} + 6y(t) = 2 \frac{du(t)}{dt} + 1
$$


Here:
- $y(t)$: Output signal
- $u(t)$: Input signal

---

### Step 2: Apply the Laplace Transform
Taking the Laplace transform (with zero initial conditions), we get:


$$
s^2 Y(s) + 5s Y(s) + 6Y(s) = 2s U(s) + 1
$$


Where:
- $Y(s)$: Laplace transform of $y(t)$
- $U(s)$: Laplace transform of $u(t)$

---

### Step 3: Solve for the Transfer Function
Rearrange to express $Y(s)$ in terms of $U(s)$:


$$
Y(s) \left(s^2 + 5s + 6\right) = 2s U(s) + 1
$$


Divide through by the denominator to get the transfer function:


$$
\frac{Y(s)}{U(s)} = \frac{2s + 1}{s^2 + 5s + 6}
$$


---

### Step 4: Analyze Poles and Zeros
The transfer function is:


$$
H(s) = \frac{2s + 1}{s^2 + 5s + 6}
$$


1. **Zeros**: The zeros are the roots of the numerator $2s + 1 = 0$.
   
   $$\text{Solve: } 2s + 1 = 0 \implies s = -\frac{1}{2}
   $$
   - Zero: $s = -\frac{1}{2}$

2. **Poles**: The poles are the roots of the denominator $s^2 + 5s + 6 = 0$.
   
   $$\text{Factorize: } s^2 + 5s + 6 = (s + 2)(s + 3)$$

   $$\text{Solve: } s + 2 = 0 \implies s = -2, \quad s + 3 = 0 \implies s = -3$$
   
   
   - Poles: $s = -2$, $s = -3$

---

### Step 5: Interpretation
- **Poles**: (s = -2) and (s = -3) determine the system's stability and response characteristics. Since both poles have negative real parts, the system is stable.
- **Zero**: $s = -\frac{1}{2}$ influences the frequency response of the system by introducing a notch at this location.

---

### Final Answer
- **Poles**: $s = -2$, $s = -3$
- **Zero**: $s = -\frac{1}{2}$

> The reason other responses consider the +1 a term independent of U(s) and discard it when calculating the zero, making it s = 0.

This happens due to **different interpretations of the input-output relationship** in the given differential equation. Let me explain why some responses might discard the constant term +1+1 when calculating the zero.

### The Key Difference

The differential equation is:

$$
\frac{d^2y(t)}{dt^2} + 5\frac{dy(t)}{dt} + 6y(t) = 2\frac{du(t)}{dt} + 1
$$

When taking the Laplace transform, the right-hand side becomes:

$$2sU(s)+ 1$$

Now, the debate arises: **Should the constant term +1 be treated as part of the input U(s) or as an independent external forcing term?**

> Two Interpretations:

1. **Include +1 as part of the forcing function:**
    
    - In this case, 11 is treated as a separate input independent of U(s)U(s).
    - The transfer function is derived solely based on the response due to U(s)U(s), so 11 is ignored when calculating zeros. This would lead to the numerator being 2s2s, making the **zero** s=0s = 0.
2. **Treat +1 as part of the same input signal:**
    
    - Here, the constant term +1+1 is lumped with U(s)U(s), as done in the original calculation. This leads to the numerator 2s+12s + 1, and the zero is calculated by solving 2s+1=02s + 1 = 0, resulting in s=−12s = -\frac{1}{2}.

---

> Why s=0s = 0 is Sometimes Assumed

The main reason is **how the transfer function is defined**:

- A transfer function, H(s), typically assumes that U(s) is the only input and ignores any independent forcing terms.
- This approach isolates the system’s response due to U(s), making the numerator 2s, and hence, the zero is s=0.

---

### Why s=−12s = -\frac{1}{2} is Valid

In the full context of the given problem, where 11 is explicitly included as part of the forcing term, it makes sense to incorporate +1+1 into the numerator calculation. This leads to the zero being s=−12s = -\frac{1}{2}.

---

### Which Interpretation is Correct?

It depends on the context:

- If the goal is to analyze the system's response **specifically to U(s)U(s)** as an input, s=0s = 0 may be a valid zero.
- If the equation is interpreted holistically, treating 11 as part of the forcing term, s=−12s = -\frac{1}{2} is more appropriate.

Both interpretations are valid, but the assumptions behind each should be made clear.

Would you like clarification on how to interpret this for a specific type of analysis?


$/$\begin{align}
&&()
\end{align}$/$

$/$\begin{align}
&&()
\end{align}$/$

