

#### The setup and form
$$\begin{align}
& \frac{2x+1}{(x+1)(x+2)} = \frac{A}{(x+1)} + \frac{B}{(x+2)} + \frac{C}{(x+2)^2} &(i)
\\\\
& \frac{2x+1}{(x+1)(x^2+2)} = \frac{A}{x+1} + \frac{Bx+C}{x^2+2} &(ii)
\\\\
& \frac{2x+1}{(x+1)(x)^2} = \frac{A}{x+1} + \frac{B}{x} + \frac{C}{x^2} &(iii)
\\\\
& \frac{2x+1}{(x+1)(x^4)} = \frac{A}{x+1}+\frac{B}{x}+\frac{C}{x^2}+\frac{D}{x^3}+\frac{E}{x^4} &(iv)
\end{align}$$


#### The _Cover-up_ method

The method involves picking the constant you want to solve for, removing it's denominator from the original equation and making _x_ equal to the value it would take to make that denominator _=0_.

**Example:**

$$\begin{align}
& \frac{2x+1}{(x+1)(x+2)} = \frac{A}{(x+1)} + \frac{B}{(x+2)} + \frac{C}{(x+2)^2} &(1)
\end{align}$$

Solving for B, we must _"cover-up"_ (x+2) from the original equation and let x=-2:

$$\begin{align}
& \frac{2x+1}{(x+1)} = B &(2)
\\\\
& \frac{2(-2)+1}{(-2)+1} = B &(3)
\\\\
& 3 = B &(4)
\end{align}$$


